Condense and conclude talk

experiments/Tree_Traversal.thy
@@ -21,32 +21,32 @@ definition [applicative_unfold]: "liftSt2 f x y = Pair f \<diamond> x \<diamond>
 
 definition "fresh n = (n, n + 1)"
 
-primrec label_tree :: "'a tree \<Rightarrow> nat \<Rightarrow> nat tree \<times> nat"
+primrec number_tree :: "'a tree \<Rightarrow> nat \<Rightarrow> nat tree \<times> nat"
 where
-    "label_tree (Leaf _) = liftSt1 Leaf fresh"
-  | "label_tree (Node l r) = liftSt2 Node (label_tree l) (label_tree r)"
+    "number_tree (Leaf _) = liftSt1 Leaf fresh"
+  | "number_tree (Node l r) = liftSt2 Node (number_tree l) (number_tree r)"
 
-primrec label_list :: "'a list \<Rightarrow> nat \<Rightarrow> nat list \<times> nat"
+primrec number_list :: "'a list \<Rightarrow> nat \<Rightarrow> nat list \<times> nat"
 where
-    "label_list [] = pure []"
-  | "label_list (x # xs) = liftSt2 (op #) fresh (label_list xs)"
+    "number_list [] = pure []"
+  | "number_list (x # xs) = liftSt2 (op #) fresh (number_list xs)"
 
-lemma label_append: "label_list (a @ b) = liftSt2 (op @) (label_list a) (label_list b)"
+lemma label_append: "number_list (a @ b) = liftSt2 (op @) (number_list a) (number_list b)"
 proof (induction a)
   case Nil
-  have "label_list b = liftSt2 (op @) (pure []) (label_list b)"
+  have "number_list b = liftSt2 (op @) (pure []) (number_list b)"
     by applicative_lifting simp
   thus ?case by simp
 next
   case (Cons a1 a2)
-  let ?la2 = "label_list a2"
-  let ?lb = "label_list b"
+  let ?la2 = "number_list a2"
+  let ?lb = "number_list b"
   have "liftSt2 (op #) fresh (liftSt2 (op @) ?la2 ?lb) = liftSt2 (op @) (liftSt2 (op #) fresh ?la2) ?lb"
     by applicative_lifting simp
   thus ?case using Cons.IH by simp
 qed
 
-lemma label_tree_list: "liftSt1 labels (label_tree t) = label_list (labels t)"
+lemma number_tree_list: "liftSt1 labels (number_tree t) = number_list (labels t)"
 proof (induction t)
   case (Leaf x)
   have "liftSt1 labels (liftSt1 Leaf fresh) = liftSt2 (op #) fresh (Pair [])"
@@ -54,11 +54,31 @@ proof (induction t)
   thus ?case by simp
 next
   case (Node l r)
-  let ?ll = "liftSt1 labels (label_tree l)"
-  let ?lr = "liftSt1 labels (label_tree r)"
-  have "liftSt1 labels (liftSt2 Node (label_tree l) (label_tree r)) = liftSt2 (op @) ?ll ?lr"
+  let ?ll = "liftSt1 labels (number_tree l)"
+  let ?lr = "liftSt1 labels (number_tree r)"
+  have "liftSt1 labels (liftSt2 Node (number_tree l) (number_tree r)) = liftSt2 (op @) ?ll ?lr"
     by applicative_lifting simp
   thus ?case using Node.IH by (simp add: label_append)
 qed
+
+experiment begin
+lemmas [simp] = liftSt1_def liftSt2_def
+
+lemma "Pair labels \<diamond> number_tree t = number_list (labels t)"
+proof (induction t)
+  case (Leaf x)
+  have "Pair labels \<diamond> (Pair Leaf \<diamond> fresh) = Pair op # \<diamond> fresh \<diamond> Pair []"
+    by applicative_lifting simp
+  thus ?case by simp
+next
+  case (Node l r)
+  let ?ll = "Pair labels \<diamond> number_tree l"
+  let ?lr = "Pair labels \<diamond> number_tree r"
+  have "Pair labels \<diamond> (Pair Node \<diamond> number_tree l \<diamond> number_tree r) = Pair op @ \<diamond> ?ll \<diamond> ?lr"
+    by applicative_lifting simp
+  thus ?case using Node.IH by (simp add: label_append)
+qed
+
+end
 
 end
